Weidenbach_Book/IsaSAT_Setup.thy
@@ -96,21 +96,22 @@ lemma incr_decision_hnr[sepref_fr_rules]:
 paragraph \<open>Base state\<close>
 
 type_synonym minimize_assn = \<open>minimize_status array \<times> uint32 array \<times> nat\<close>
+type_synonym out_learned = \<open>nat clause_l\<close>
 
 type_synonym twl_st_wll_trail =
   \<open>trail_pol_assn \<times> clauses_wl \<times> nat \<times> option_lookup_clause_assn \<times>
     lit_queue_l \<times> watched_wl \<times> vmtf_remove_assn \<times> phase_saver_assn \<times>
-    uint32 \<times> minimize_assn \<times> lbd_assn \<times> stats\<close>
+    uint32 \<times> minimize_assn \<times> lbd_assn \<times> out_learned_assn \<times> stats\<close>
 
 text \<open>\<^emph>\<open>heur\<close> stands for heuristic.\<close>
 type_synonym twl_st_wl_heur =
   \<open>(nat,nat)ann_lits \<times> nat clause_l list \<times> nat \<times>
     nat clause option \<times> nat lit_queue_wl \<times> nat list list \<times> vmtf_remove_int \<times> bool list \<times>
-    nat \<times> nat conflict_min_cach \<times> lbd \<times> stats\<close>
+    nat \<times> nat conflict_min_cach \<times> lbd \<times> out_learned \<times> stats\<close>
 
 type_synonym twl_st_wl_heur_trail_ref =
   \<open>trail_pol \<times> nat clause_l list \<times> nat \<times> nat cconflict \<times> nat lit_queue_wl \<times> nat list list \<times>
-   vmtf_remove_int \<times> bool list \<times> nat \<times> nat conflict_min_cach \<times> lbd \<times> stats\<close>
+   vmtf_remove_int \<times> bool list \<times> nat \<times> nat conflict_min_cach \<times> lbd \<times> out_learned \<times> stats\<close>
 
 fun get_clauses_wl_heur :: \<open>twl_st_wl_heur \<Rightarrow> nat clauses_l\<close> where
   \<open>get_clauses_wl_heur (M, N, U, D, _) = N\<close>
@@ -139,6 +140,9 @@ fun get_conflict_cach:: \<open>twl_st_wl_heur \<Rightarrow> nat conflict_min_cac
 fun get_lbd :: \<open>twl_st_wl_heur \<Rightarrow> lbd\<close> where
   \<open>get_lbd (_, _, _, _, _, _, _, _, _, _, lbd, _) = lbd\<close>
 
+fun get_outlearned :: \<open>twl_st_wl_heur \<Rightarrow> out_learned\<close> where
+  \<open>get_outlearned (_, _, _, _, _, _, _, _, _, _, _, out, _) = out\<close>
+
 abbreviation phase_saver_conc where
   \<open>phase_saver_conc \<equiv> array_assn bool_assn\<close>
 
@@ -151,7 +155,7 @@ definition cach_refinement_empty where
 
 definition twl_st_heur :: \<open>(twl_st_wl_heur \<times> nat twl_st_wl) set\<close> where
 \<open>twl_st_heur =
-  {((M', N', U', D', Q', W', vm, \<phi>, clvls, cach, lbd, stats), (M, N, U, D, NE, UE, Q, W)).
+  {((M', N', U', D', Q', W', vm, \<phi>, clvls, cach, lbd, outl, stats), (M, N, U, D, NE, UE, Q, W)).
     M = M' \<and> N' = N \<and> U' = U \<and>
     D' = D \<and>
      Q' = Q \<and>
@@ -160,7 +164,8 @@ definition twl_st_heur :: \<open>(twl_st_wl_heur \<times> nat twl_st_wl) set\<cl
     phase_saving \<phi> \<and>
     no_dup M \<and>
     clvls \<in> counts_maximum_level M D \<and>
-    cach_refinement_empty cach
+    cach_refinement_empty cach \<and>
+    out_learned M D outl
   }\<close>
 
 definition twl_st_heur_assn :: \<open>twl_st_wl_heur \<Rightarrow> twl_st_wll_trail \<Rightarrow> assn\<close> where
@@ -173,18 +178,31 @@ definition twl_st_heur_assn :: \<open>twl_st_wl_heur \<Rightarrow> twl_st_wll_tr
   uint32_nat_assn *a
   cach_refinement_assn *a
   lbd_assn *a
+  out_learned_assn *a
   stats_assn\<close>
 
 definition twl_st_assn :: \<open>nat twl_st_wl \<Rightarrow> twl_st_wll_trail \<Rightarrow> assn\<close> where
 \<open>twl_st_assn = hr_comp twl_st_heur_assn twl_st_heur\<close>
 
-type_synonym twl_st_heur_pol_no_clvls =
-  \<open>trail_pol_assn \<times> clauses_wl \<times> nat \<times> option_lookup_clause_assn \<times>
-    lit_queue_l \<times> watched_wl \<times> vmtf_remove_assn \<times> phase_saver_assn \<times> uint32 \<times>
-    minimize_assn \<times> lbd_assn \<times> stats\<close>
+definition (in isasat_input_ops) twl_st_heur_no_clvls
+  :: \<open>(twl_st_wl_heur \<times> nat twl_st_wl) set\<close>
+where
+\<open>twl_st_heur_no_clvls =
+  {((M', N', U', D', Q', W', vm, \<phi>, clvls, cach, lbd, outl, stats), (M, N, U, D, NE, UE, Q, W)).
+    M = M' \<and> N' = N \<and> U' = U \<and>
+    D' = D \<and>
+     Q' = Q \<and>
+    (W', W) \<in> \<langle>Id\<rangle>map_fun_rel D\<^sub>0 \<and>
+    vm \<in> vmtf M \<and>
+    phase_saving \<phi> \<and>
+    no_dup M \<and>
+    cach_refinement_empty cach \<and>
+    out_learned_confl M D outl
+  }\<close>
 
+(* TODO Kill *)
 definition twl_st_heur_pol_assn
-  :: \<open>twl_st_wl_heur_trail_ref \<Rightarrow> twl_st_heur_pol_no_clvls \<Rightarrow> assn\<close>
+  :: \<open>twl_st_wl_heur_trail_ref \<Rightarrow> twl_st_wll_trail \<Rightarrow> assn\<close>
 where
   \<open>twl_st_heur_pol_assn =
     trail_pol_assn *a clauses_ll_assn *a nat_assn *a
@@ -195,11 +213,12 @@ where
     uint32_nat_assn *a
     cach_refinement_assn *a
     lbd_assn *a
+    out_learned_assn *a
     stats_assn\<close>
 
 definition (in isasat_input_ops) twl_st_heur_pol :: \<open>(twl_st_wl_heur_trail_ref \<times> nat twl_st_wl) set\<close> where
 \<open>twl_st_heur_pol =
-  {((M', N', U', D', Q', W', vm, \<phi>, clvls, cach, lbd), (M, N, U, D, NE, UE, Q, W)).
+  {((M', N', U', D', Q', W', vm, \<phi>, clvls, cach, lbd, outl, stats), (M, N, U, D, NE, UE, Q, W)).
     (M', M) \<in> trail_pol \<and> N' = N \<and> U' = U \<and> D = D' \<and>
      Q' = Q \<and>
     (W', W) \<in> \<langle>Id\<rangle>map_fun_rel D\<^sub>0 \<and>
@@ -207,17 +226,18 @@ definition (in isasat_input_ops) twl_st_heur_pol :: \<open>(twl_st_wl_heur_trail
     phase_saving \<phi> \<and>
     no_dup M \<and>
     clvls \<in> counts_maximum_level M D \<and>
-    cach_refinement_empty cach
+    cach_refinement_empty cach \<and>
+    out_learned M D' outl
   }\<close>
 
 lemma twl_st_heur_pol_alt_def:
   \<open>twl_st_heur_pol =
-    (trail_pol \<times>\<^sub>r Id \<times>\<^sub>r nat_rel \<times>\<^sub>r Id \<times>\<^sub>r Id \<times>\<^sub>r Id \<times>\<^sub>r Id \<times>\<^sub>r Id \<times>\<^sub>r Id \<times>\<^sub>r Id) O twl_st_heur\<close>
+    (trail_pol \<times>\<^sub>r Id \<times>\<^sub>r nat_rel \<times>\<^sub>r Id \<times>\<^sub>r Id \<times>\<^sub>r Id \<times>\<^sub>r Id \<times>\<^sub>r Id \<times>\<^sub>r Id \<times>\<^sub>r Id \<times>\<^sub>r Id) O twl_st_heur\<close>
   by (force simp: twl_st_heur_pol_def twl_st_heur_def)
 
 lemma twl_st_heur_pol_assn_twl_st_heur_assn:
   \<open>hr_comp twl_st_heur_pol_assn
-    (trail_pol \<times>\<^sub>r Id \<times>\<^sub>r nat_rel \<times>\<^sub>r Id \<times>\<^sub>r Id \<times>\<^sub>r Id \<times>\<^sub>r Id \<times>\<^sub>r Id \<times>\<^sub>r Id \<times>\<^sub>r Id) =
+    (trail_pol \<times>\<^sub>r Id \<times>\<^sub>r nat_rel \<times>\<^sub>r Id \<times>\<^sub>r Id \<times>\<^sub>r Id \<times>\<^sub>r Id \<times>\<^sub>r Id \<times>\<^sub>r Id \<times>\<^sub>r Id \<times>\<^sub>r Id) =
      twl_st_heur_assn\<close>
   unfolding twl_st_heur_pol_assn_def twl_st_heur_assn_def
   by simp
@@ -231,7 +251,7 @@ lemma twl_st_heur_assn_assn:
 type_synonym (in -) twl_st_wl_heur_W_list =
   \<open>(nat,nat) ann_lits \<times> nat clause_l list \<times> nat \<times>
     nat cconflict \<times> nat literal list \<times> nat list list \<times> vmtf_remove_int \<times> bool list \<times> nat \<times>
-    nat conflict_min_cach \<times> lbd \<times> stats\<close>
+    nat conflict_min_cach \<times> lbd \<times> out_learned \<times> stats\<close>
 
 
 definition twl_st_wl_heur_W_list_rel :: \<open>(twl_st_wl_heur_W_list \<times> twl_st_wl_heur) set\<close> where
@@ -247,6 +267,7 @@ definition twl_st_wl_heur_W_list_rel :: \<open>(twl_st_wl_heur_W_list \<times> t
      nat_rel \<times>\<^sub>r
      Id \<times>\<^sub>r
      Id \<times>\<^sub>r
+     Id \<times>\<^sub>r
      Id\<close>
 
 definition twl_st_heur_W_list_assn :: \<open>twl_st_wl_heur_W_list \<Rightarrow> twl_st_wll_trail \<Rightarrow> assn\<close> where
@@ -256,11 +277,11 @@ definition twl_st_heur_W_list_assn :: \<open>twl_st_wl_heur_W_list \<Rightarrow>
   (list_assn unat_lit_assn) *a
   arrayO_assn (arl_assn nat_assn) *a
   vmtf_remove_conc *a phase_saver_conc *a uint32_nat_assn *a cach_refinement_assn *a
-  lbd_assn *a stats_assn
+  lbd_assn *a out_learned_assn *a stats_assn
   )\<close>
 
 lemma twl_st_wl_heur_W_list_rel_twl_st_rel: \<open>twl_st_wl_heur_W_list_rel O twl_st_heur =
-   {((M', N', U', D', Q', W', vm, \<phi>, clvls, cach, lbd, stats), M, N, U, D, NE, UE, Q, W).
+   {((M', N', U', D', Q', W', vm, \<phi>, clvls, cach, lbd, outl, stats), M, N, U, D, NE, UE, Q, W).
      M = M' \<and>
      N' = N \<and>
      U' = U \<and>
@@ -268,7 +289,8 @@ lemma twl_st_wl_heur_W_list_rel_twl_st_rel: \<open>twl_st_wl_heur_W_list_rel O t
      (Q', Q) \<in> list_mset_rel \<and>
      (W', W) \<in> \<langle>Id\<rangle>map_fun_rel D\<^sub>0 \<and>
      vm \<in> vmtf M \<and> phase_saving \<phi> \<and> no_dup M \<and> clvls \<in> counts_maximum_level M D\<and>
-     cach_refinement_empty cach}\<close>
+     cach_refinement_empty cach \<and>
+     out_learned M D outl}\<close>
   unfolding twl_st_heur_def twl_st_wl_heur_W_list_rel_def
   by force
 
@@ -307,7 +329,7 @@ lemma literals_are_in_\<L>\<^sub>i\<^sub>n_heur_in_D\<^sub>0':
 type_synonym (in -) twl_st_wl_heur_lookup_conflict =
   \<open>(nat,nat) ann_lits \<times> nat clause_l list \<times> nat \<times>
     (bool \<times> nat \<times> bool option list) \<times> nat literal multiset \<times> nat list list \<times> vmtf_remove_int \<times>
-     bool list \<times> nat \<times> nat conflict_min_cach \<times> lbd \<times> stats\<close>
+     bool list \<times> nat \<times> nat conflict_min_cach \<times> lbd \<times> out_learned \<times> stats\<close>
 
 definition twl_st_wl_heur_lookup_lookup_clause_rel
   :: \<open>(twl_st_wl_heur_lookup_conflict \<times> twl_st_wl_heur) set\<close>
@@ -324,6 +346,7 @@ where
      nat_rel \<times>\<^sub>r
      Id \<times>\<^sub>r
      Id \<times>\<^sub>r
+     Id \<times>\<^sub>r
      Id\<close>
 
 definition twl_st_heur_lookup_lookup_clause_assn
@@ -335,7 +358,7 @@ where
     clause_l_assn *a
     arrayO_assn (arl_assn nat_assn) *a
     vmtf_remove_conc *a phase_saver_conc *a uint32_nat_assn *a cach_refinement_assn *a
-    lbd_assn *a
+    lbd_assn *a out_learned_assn *a
     stats_assn
   \<close>
 
